Worklist_Algorithms/Next_Key.thy
@@ -39,7 +39,7 @@ lemma hm_it_next_key_rule:
       apply sep_auto
       subgoal for a b list aa ba
         apply (rule weak_map_of_SomeI[of _ b])
-        apply auto
+        apply clarsimp
         apply (rule bexI[of _ "l ! i"])
         subgoal
           by (metis list.set_intros(1))
@@ -49,11 +49,6 @@ lemma hm_it_next_key_rule:
       done
   qed
   done
-
-lemma
-  "<P * R> c <\<lambda> r. Q r * R>" if "<P> c <\<lambda> r. Q r>"
-  using that
-  by (simp add: frame_rule)
 
 
 definition
@@ -65,8 +60,7 @@ definition
   "
 
 lemma hm_it_next_key_next_key_aux:
-  fixes K :: "_ :: {hashable, heap} \<Rightarrow> _"
-  assumes "CONSTRAINT is_pure K" "nofail (next_key m)"
+  assumes "is_pure K" "nofail (next_key m)"
   shows
     "<hm.assn K V m mi>
       hm_it_next_key mi
@@ -85,7 +79,7 @@ lemma hm_it_next_key_next_key_aux:
       from prems obtain k v where "m k = Some v" "(x, k) \<in> the_pure K" "(v', v) \<in> the_pure V"
         apply atomize_elim
         by (meson map_rel_obtain2)
-      with prems \<open>CONSTRAINT is_pure K\<close> show ?thesis
+      with prems \<open>is_pure K\<close> show ?thesis
         apply -
         apply (rule exI[where x = k], rule exI[where x = m'])
         apply sep_auto
@@ -97,15 +91,12 @@ lemma hm_it_next_key_next_key_aux:
   done
 
 lemma hm_it_next_key_next_key:
-  fixes K :: "_ :: {hashable, heap} \<Rightarrow> _"
   assumes "CONSTRAINT is_pure K"
-  shows
-    "(hm_it_next_key, next_key) \<in> (hm.assn K V)\<^sup>k \<rightarrow>\<^sub>a K"
+  shows "(hm_it_next_key, next_key) \<in> (hm.assn K V)\<^sup>k \<rightarrow>\<^sub>a K"
   using assms by sepref_to_hoare (sep_auto intro!: hm_it_next_key_next_key_aux)
 
 lemma hm_it_next_key_next_key':
-  shows
-    "(hm_it_next_key, next_key) \<in> (hm.hms_assn V)\<^sup>k \<rightarrow>\<^sub>a id_assn"
+  "(hm_it_next_key, next_key) \<in> (hm.hms_assn V)\<^sup>k \<rightarrow>\<^sub>a id_assn"
   unfolding hm.hms_assn_def
   apply sepref_to_hoare
   apply sep_auto
@@ -117,10 +108,78 @@ lemma hm_it_next_key_next_key':
           and Q = "\<lambda> x. is_hashmap mi m' * \<up> (x \<in> dom mi) * map_assn V m mi"]
         )
       apply (sep_auto; unfold map_assn_def; auto; fail)+
-    apply (rule norm_pre_pure_rule1)
-    apply (rule frame_rule[OF hm_it_next_key_rule[of mi m']])
-    by (sep_auto; unfold map_assn_def; auto)+
+    by (rule norm_pre_pure_rule1, rule frame_rule[OF hm_it_next_key_rule[of mi m']]) sep_auto
   done
+
+lemma no_fail_next_key_iff:
+  "nofail (next_key m) \<longleftrightarrow> m \<noteq> Map.empty"
+  unfolding next_key_def by auto
+
+context
+  fixes mi m K
+  assumes map_rel: "(mi, m) \<in> \<langle>K, Id\<rangle>map_rel"
+begin
+
+private lemma k_aux:
+  assumes "k \<in> dom mi" "(mi, m) \<in> \<langle>K, Id\<rangle>map_rel"
+  shows "\<exists> k'. (k, k') \<in> K"
+  using assms unfolding map_rel_def by auto
+
+private lemma k_aux2:
+  assumes "k \<in> dom mi" "(k, k') \<in> K"
+  shows "k' \<in> dom m"
+  using assms map_rel unfolding map_rel_def by (cases "m k'") (auto dest: fun_relD)
+
+private lemma map_empty_iff: "mi \<noteq> Map.empty \<longleftrightarrow> m \<noteq> Map.empty"
+  using map_rel by auto
+
+private lemma aux:
+  assumes "RETURN k \<le> next_key mi"
+  shows "RETURN (SOME k'. (k, k') \<in> K) \<le> next_key m"
+  using map_rel assms
+  unfolding next_key_def
+  apply (cases "m \<noteq> Map.empty")
+   apply (clarsimp simp: map_empty_iff)
+  apply (frule (1) k_aux[OF domI])
+  apply (drule someI_ex)
+  apply (auto dest: k_aux2[OF domI])
+  done
+
+private lemma aux1:
+  assumes "RETURN k \<le> next_key mi" "nofail (next_key m)"
+  shows "(k, SOME k'. (k, k') \<in> K) \<in> K"
+  using map_rel assms
+  unfolding next_key_def
+  apply (cases "m \<noteq> Map.empty")
+   apply (auto simp: map_empty_iff)
+  apply (drule (1) k_aux[OF domI], erule someI_ex)
+  done
+
+lemmas hm_it_next_key_next_key''_aux = aux aux1
+
+end (* Anonymous context *)
+
+lemma hm_it_next_key_next_key'':
+  assumes "is_pure K"
+  shows "(hm_it_next_key, next_key) \<in> (hm.hms_assn' K V)\<^sup>k \<rightarrow>\<^sub>a K"
+  unfolding hm.hms_assn'_def
+  apply sepref_to_hoare
+  unfolding hr_comp_def
+  apply sep_auto
+  subgoal for m m' mi
+    using hm_it_next_key_next_key'[to_hnr, unfolded hn_refine_def, of mi V m']
+    apply (sep_auto simp: hn_ctxt_def)
+    subgoal
+      unfolding no_fail_next_key_iff by auto
+    apply (erule cons_post_rule)
+    using \<open>is_pure K\<close>
+    apply sep_auto
+     apply (erule (1) hm_it_next_key_next_key''_aux)
+    apply (subst pure_the_pure[symmetric, of K], assumption)
+    apply (sep_auto intro: hm_it_next_key_next_key''_aux simp: pure_def)
+    done
+  done
+
 
 subsection \<open>Computing the range of a map\<close>
 
@@ -161,14 +220,9 @@ lemma ran_of_map_correct[refine]:
   "ran_of_map m \<le> SPEC (\<lambda> r. set r = ran m)" if "finite (dom m)"
   using that unfolding ran_of_map_def next_key_def
   apply (refine_vcg wf_ran_of_map_var)
-         apply (simp; fail)
-        apply (simp; fail)
-       apply (simp; fail)
-      apply (clarsimp; fail)
-     apply (clarsimp; fail)
+         apply (clarsimp; fail)+
   subgoal for s xs m' x v xs' xs1 xs'1
-    unfolding dom_def
-    by (clarsimp simp: map_upd_eq_restrict, auto dest: insert_restrict_ran)
+    unfolding dom_def by (clarsimp simp: map_upd_eq_restrict, auto dest: insert_restrict_ran)
   subgoal
     unfolding ran_of_map_var_def op_map_extract_def by (fastforce intro: card_Diff1_less)
   by auto
@@ -204,16 +258,33 @@ lemma [intf_of_assn]:
   by simp
 
 context
-  notes [sepref_fr_rules] = hm_it_next_key_next_key'[folded hm.hms_assn'_id_hms_assn]
+  fixes K :: "_ \<Rightarrow> _ :: {hashable, heap} \<Rightarrow> assn"
+  assumes is_pure_K[safe_constraint_rules]: "is_pure K"
+  and left_unique_K[safe_constraint_rules]: "IS_LEFT_UNIQUE (the_pure K)"
+  and right_unique_K[safe_constraint_rules]: "IS_RIGHT_UNIQUE (the_pure K)"
+  notes [sepref_fr_rules] = hm_it_next_key_next_key''[OF is_pure_K]
 begin
 
 sepref_definition ran_of_map_impl is
+  "ran_of_map" :: "(hm.hms_assn' K A)\<^sup>d \<rightarrow>\<^sub>a list_assn A"
+  unfolding ran_of_map_def hm.hms_assn'_id_hms_assn[symmetric]
+  unfolding op_map_is_empty_def[symmetric]
+  unfolding hm.hms_fold_custom_empty HOL_list.fold_custom_empty
+  by sepref
+
+end (* Anonymous context for setup *)
+
+context
+  notes [sepref_fr_rules] = hm_it_next_key_next_key'[folded hm.hms_assn'_id_hms_assn]
+begin
+
+sepref_definition ran_of_map_impl' is
   "ran_of_map" :: "(hm.hms_assn A)\<^sup>d \<rightarrow>\<^sub>a list_assn A"
   unfolding ran_of_map_def hm.hms_assn'_id_hms_assn[symmetric]
   unfolding op_map_is_empty_def[symmetric]
   unfolding hm.hms_fold_custom_empty HOL_list.fold_custom_empty
   by sepref
 
-end (* End of anonymous context for setup *)
+end (* Anonymous context for setup *)
 
 end (* Theory *)
